FromAxioms/NumberTheory.lean
@@ -14,3 +14,4 @@ import FromAxioms.NumberTheory.Arith
 import FromAxioms.NumberTheory.Integer
 import FromAxioms.NumberTheory.Prime
 import FromAxioms.NumberTheory.Rational
+import FromAxioms.NumberTheory.Congruence
